src/named/egraph/UFProofs.v
@@ -161,21 +161,6 @@ Section WithVar.
   Notation pfM := (stateT proof_context option).
 
   (*TODO: move to Monad.v*)
-  
-Notation "'let' p <^- e 'in' b" :=
-  (Mbind (fun p => b) (lift e))
-    (in custom monadic_do at level 200, left associativity, p pattern at level 0, e constr, b custom monadic_do).
-
-
-  Notation "'ret' { M } e" := (Mret (M:=M) e) (in custom monadic_do at level 90, e constr).
-
-Notation "'let' { M } p <- e 'in' b" :=
-  (Mbind (M:=M) (fun p => b) e)
-    (in custom monadic_do at level 200, left associativity, p pattern at level 0, e constr, b custom monadic_do).
-
-Notation "'let' { M } p <?- e 'in' b" :=
-  (Mbind (M:=M) (fun x => match x with p => b | _ => default end) e)
-    (in custom monadic_do at level 200, left associativity, p pattern at level 0, e constr, b custom monadic_do).
 
 Instance stateT_default S M A `{WithDefault (M (A*S))%type}
   : WithDefault (stateT S M A) :=
@@ -763,7 +748,47 @@ Existing  Instance stateT_trans.
           erewrite lookup_sort'_forest_subrel; eauto.
         }
       Qed.
+
+       
+      Lemma lookup_term_forest_subrel' f f' pc1 pc2 e
+        : forest_subrel f' f ->
+          uf_ok pc1.(id_equiv) f ->
+          uf_ok pc2.(id_equiv) f' ->
+          pc1.(hashcons) = pc2.(hashcons) ->
+          forall i,
+            Some i = lookup_term pc1 e ->
+            exists j, equiv_by_forest f i j
+                      /\ Some j = lookup_term pc2 e.
+      Proof.
+        intros Hsub Hokf Hokf';
+          induction e;
+          intros; simpl in *.
+        {
+          destruct pc1; destruct pc2; simpl in *; subst.
+          (*
+          now auto.
+        revert H1; 
+          case_match;[| congruence].
         
+        enough (Some l1 = list_Mmap (lookup_term pc2) l0) as H'.
+        {
+          rewrite<- H'.
+          congruence.
+        }
+        revert dependent l1.
+        revert dependent l0.
+        induction l0;
+          intros; simpl in *; auto.
+        break.
+        revert HeqH1.
+        case_match;[| congruence].
+        case_match;[| congruence].
+        intro H'; safe_invert H'.
+        specialize (H H0 p eq_refl).
+        rewrite <- H.
+        erewrite <- IHl0; eauto.
+      Qed.*)
+      Abort.
 
       Lemma find_ok pc f pc' (i i' : positive)
         : proof_context_valid pc f ->
@@ -797,6 +822,22 @@ Existing  Instance stateT_trans.
         fun pc =>
           @! let (uf', i') <- union pc.(id_equiv) i1 i2 in
             ret (i',MkPC uf' pc.(hashcons)).
+
+      
+      Lemma points_to_tree_union_l x0 x1
+        : points_to (tree_union_l x0 x1) = points_to x0.
+      Proof.
+        destruct x0; auto.
+      Qed.
+      Hint Rewrite points_to_tree_union_l : utils.
+
+      Lemma points_to_in_same x0
+        : In_tree (points_to x0) x0 <-> True.
+      Proof.
+        destruct x0; simpl; intuition auto.
+      Qed.
+      Hint Rewrite points_to_in_same : utils.
+        
       
       Lemma union_ok pc f pc' i' (i1 i2 : positive)
         : proof_context_valid pc f ->
@@ -815,10 +856,39 @@ Existing  Instance stateT_trans.
         revert HeqH0.
         intro.
         destruct H; simpl in *.
+        pose proof HeqH0.
         eapply union_spec in HeqH0; eauto.
         break.
-        eexists; intuition eauto.
-        constructor; intuition eauto.
+        destruct HeqH0.
+        {
+          break; subst.
+          exists f; subst; intuition eauto;
+              try exact (fun a b c => c);
+              constructor; simpl; eauto.  
+        }
+        break.
+        exists (tree_union_l x0 x1 :: x).
+        intuition subst.
+        1:admit (*permutation x union -> subrel*).
+        {
+          rewrite points_to_tree_union_l.
+          exists (tree_union_l x0 x1);
+            basic_utils_crush.
+          all: admit.
+        }
+        {
+          rewrite points_to_tree_union_l.
+          exists (tree_union_l x0 x1);
+            basic_utils_crush.
+          all: admit.
+        }
+        {          
+          constructor; intuition eauto.
+          { eapply H0; eauto.
+            eapply lookup_sort_forest_subrel; cycle 4; eauto.
+            (*
+            TODO: subrel wrong direction
+            TODO: wrong uf
         {
           eapply H0.
           eapply lookup_sort_forest_subrel; cycle 4.
@@ -899,419 +969,10 @@ Existing  Instance stateT_trans.
           case_match;[| congruence].
           
         }
-        
+             *)
+            Abort.
 
-  Section WithProofCtx.
-    Context (pc : proof_context).
-
-    (*TODO: make i the canonical node*)
-    Definition node_at n i :=      
-      Some i = map.get pc.(hashcons) n.
-
-     (*
-  Inductive eq_sort : ctx -> sort -> sort -> Prop :=
-  | eq_sort_by : forall c name t1 t2,
-      In (name, sort_eq_rule c t1 t2) l ->
-      eq_sort c t1 t2
-  | eq_sort_subst : forall c s1 s2 c' t1' t2',
-      (* Need to assert wf_ctx c here to satisfy
-         assumptions' presuppositions
-       *)
-      wf_ctx c' ->
-      eq_subst (Model:= mut_mod eq_sort eq_term wf_sort wf_term) c c' s1 s2 ->
-      eq_sort c' t1' t2' ->
-      eq_sort c t1'[/s1/] t2'[/s2/]
-  | eq_sort_refl : forall c t,
-      wf_sort c t ->
-      eq_sort c t t
-  | eq_sort_trans : forall c t1 t12 t2,
-      eq_sort c t1 t12 ->
-      eq_sort c t12 t2 ->
-      eq_sort c t1 t2
-  | eq_sort_sym : forall c t1 t2, eq_sort c t1 t2 -> eq_sort c t2 t1
-  with eq_term : ctx -> sort -> term -> term -> Prop :=
-  | eq_term_subst : forall c s1 s2 c' t e1 e2,
-      (* Need to assert wf_ctx c' here to satisfy
-         assumptions' presuppositions
-       *)
-      wf_ctx c' ->
-      eq_subst (Model:= mut_mod eq_sort eq_term wf_sort wf_term) c c' s1 s2 ->
-      eq_term c' t e1 e2 ->
-      eq_term c t[/s2/] e1[/s1/] e2[/s2/]
-  | eq_term_by : forall c name t e1 e2,
-      In (name,term_eq_rule c e1 e2 t) l ->
-      eq_term c t e1 e2
-  | eq_term_refl : forall c e t,
-      wf_term c e t ->
-      eq_term c t e e
-  | eq_term_trans : forall c t e1 e12 e2,
-      eq_term c t e1 e12 ->
-      eq_term c t e12 e2 ->
-      eq_term c t e1 e2
-  | eq_term_sym : forall c t e1 e2, eq_term c t e1 e2 -> eq_term c t e2 e1
-  (* Conversion:
-
-c |- e1 = e2 : t 
-               ||
-c |- e1 = e2 : t'
-   *)
-  | eq_term_conv : forall c t t',
-      eq_sort c t t' ->
-      forall e1 e2,
-        eq_term c t e1 e2 ->
-        eq_term c t' e1 e2
-                (*
-  (* TODO: do I want to allow implicit elements in substitutions? *)
-  (* TODO: do I want to define this in terms of eq_args? *)
-  with eq_subst : ctx -> ctx -> subst -> subst -> Prop :=
-  | eq_subst_nil : forall c, eq_subst c [] [] []
-  | eq_subst_cons : forall c c' s1 s2,
-      eq_subst c c' s1 s2 ->
-      forall name t e1 e2,
-        (* assumed because the output ctx is wf: fresh name c' ->*)
-        eq_term c t[/s2/] e1 e2 ->
-        eq_subst c ((name, t)::c') ((name,e1)::s1) ((name,e2)::s2)*)*)
-
-    (*TODO:
-      1. conversion/node id equivalence
-      2. ids for ctxs & types; do I need them?
-         - don't need ctxs since always working in 1 ctx
-         - don't need sorts since the sort is unambiguous up to union-find
-         + should be a relevant lemma in matches
-         - do I need to add sorts to egraph for the above to work?
-     *)
-  Inductive wf_term : ctx -> term -> sort -> positive -> Prop :=
-  | wf_term_by : forall c n s args c' t si i,
-      In (n, term_rule c' args t) l ->
-      wf_args c s c' si ->
-      node_at (ncon n si) i ->
-      wf_term c (con n s) t[/(with_names_from c' s)/] i
-  | wf_term_conv : forall c e t t' i i',
-      (* We add this condition so that we satisfy the assumptions of eq_sort
-         TODO: necessary? not based on current judgment scheme.
-         wf_term c e t should imply wf_sort c t,
-         and eq_sort c t t' should imply wf_sort c t
-
-
-      wf_sort c t -> 
-       *)
-      wf_term c e t i ->
-      wf_sort c t i' ->
-      wf_sort c t' i' ->
-      (*eq_sort c t t' ->*)
-      wf_term c e t' i
-  | wf_term_var : forall c n t i,
-      In (n, t) c ->
-      node_at (nvar n) i ->
-      wf_term c (var n) t i
-  with wf_sort : ctx -> sort -> positive -> Prop :=
-  | wf_sort_by : forall c n s args c' si i,
-      In (n, (sort_rule c' args)) l ->
-      wf_args c s c' si ->
-      node_at (ncon n si) i ->
-      wf_sort c (scon n s) i
-  with wf_args : ctx -> list term -> ctx -> list positive -> Prop :=
-  | wf_args_nil : forall c, wf_args c [] [] []
-  | wf_args_cons : forall c s c' name e t i li,
-      wf_term c e t[/with_names_from c' s/] i ->
-      (* these arguments are last so that proof search unifies existentials
-       from the other arguments first*)
-      wf_args c s c' li ->
-      wf_args c (e::s) ((name,t)::c') (i::li).
-
-
-
-
-
-
-
-
-    
-    (*TODO: change section name?*)
-    Context (c : ctx).
-    Context (wfl : wf_lang l).
-
-
-
-    
-       
-     (*TOOD: replace case_match with this? Copied twice already*)
-     Ltac case_match' :=
-       try lazymatch goal with
-           [ H :  context [ match ?e with
-                            | _ => _
-                            end] |- _ ] => revert H
-         end;
-       case_match.
-    
-  Section Inner.
-
-    Context (proof_result : proof_context).
-    
-    Fixpoint check_args_proof (args : list positive) (c' : ctx) :=
-      match args, c' with
-      | [], [] => Some ([],[])
-      | p::args, (_,t)::c'=>
-          @! let (lhs, rhs) <- check_args_proof args c' in
-            let (term_eq_result e1 e2 t') <?- get p proof_result in
-            (*TODO: use Eqb instance*)
-            let ! sort_eq_dec t[/with_names_from c' rhs/] t' in
-            ret (e1::lhs, e2::rhs)
-      | _,_=> None
-      end.
-
-     Definition check_node (n : node) : option node_result :=
-      match n with
-      | tn_var n =>
-          @! let t <- named_list_lookup_err c n in
-             ret (term_eq_result (var n) (var n) t)
-      | tn_con n s =>
-          @! let r <- named_list_lookup_err l n in
-             match r with
-             | term_rule c' _ t =>
-                 @! let (lhs, rhs) <- check_args_proof s c' in
-                   ret (term_eq_result (con n lhs) (con n rhs)
-                          t[/with_names_from c' rhs/])
-             | term_eq_rule c' e1 e2 t =>
-                 @! let (lhs, rhs) <- check_args_proof s c' in
-                    let lsub := with_names_from c' lhs in
-                    let rsub := with_names_from c' rhs in
-                    ret (term_eq_result e1[/lsub/] e2[/rsub/] t[/rsub/])
-             | _ => None
-             end
-      | tn_trans p0 p1 =>
-          @! let (term_eq_result e1 e2 t) <?- get p0 proof_result in
-             let (term_eq_result e1' e2' t') <?- get p1 proof_result in
-             let ! sort_eq_dec t t' in
-             let ! term_eq_dec e2 e1' in
-             ret (term_eq_result e1 e2' t)
-      | tn_sym p =>
-          @! let (term_eq_result e1 e2 t) <?- get p proof_result in
-             ret (term_eq_result e2 e1 t)
-      | tn_conv p0 p1 =>
-          @! let (sort_eq_result t1 t2) <?- get p0 proof_result in
-             let (term_eq_result e1 e2 t) <?- get p1 proof_result in
-             let ! sort_eq_dec t t1 in
-             ret (term_eq_result e1 e2 t2)
-                 
-      | sn_con n s =>
-          @! let r <- named_list_lookup_err l n in
-             match r with
-             | sort_rule c' _ =>
-                 @! let (lhs, rhs) <- check_args_proof s c' in
-                    ret (sort_eq_result (scon n lhs) (scon n rhs))
-             | sort_eq_rule c' t1 t2 =>
-                 @! let (lhs, rhs) <- check_args_proof s c' in
-                    let lsub := with_names_from c' lhs in
-                    let rsub := with_names_from c' rhs in
-                    ret (sort_eq_result t1[/lsub/] t2[/rsub/])
-             | _ => None
-             end
-      | sn_trans p0 p1 =>
-          @! let (sort_eq_result t1 t2) <?- get p0 proof_result in
-             let (sort_eq_result t1' t2') <?- get p1 proof_result in
-             let ! sort_eq_dec t2 t1' in
-             ret (sort_eq_result t1 t2')
-      | sn_sym p =>
-          @! let (sort_eq_result t1 t2) <?- get p proof_result in
-             ret (sort_eq_result t2 t1)
-      end.
-
-     
-     Definition node_result_sound res :=
-       match res with
-       | term_eq_result e1 e2 t => eq_term l c t e1 e2
-       | sort_eq_result t1 t2 => eq_sort l c t1 t2
-       end.
-
-     (* TODO: move somewhere? *)
-     Definition tree_all {A} (P : A -> Prop) t :=
-       forall n a, get n t = Some a -> P a.
-
-     Context (history_sound : tree_all node_result_sound proof_result).
-
-     
-     Lemma check_args_proof_sound args c' a1 a2
-       : check_args_proof args c' = Some (a1,a2) ->
-         eq_args l c c' a1 a2.
-     Proof.
-       revert c' a1 a2.
-       induction args; destruct c';
-         basic_goal_prep;
-         try congruence;
-         repeat case_match';
-         basic_goal_prep;
-         try congruence;
-         repeat lazymatch goal with
-           | [H : (_,_) = ( _,_) |- _ ] => safe_invert H
-           | [H : Some _ = Some _ |- _ ] => safe_invert H
-          end.
-       - constructor.
-       - constructor; eauto.
-         symmetry in HeqH1.
-         eapply history_sound in HeqH1.
-         exact HeqH1.
-       - safe_invert H.
-       - safe_invert H.
-     Qed.
-     
-     Lemma check_node_sound n res
-       : check_node n = Some res ->
-         node_result_sound res.
-     Proof.
-       destruct n;
-        basic_goal_prep;
-        (*weed out trivial goals for efficiency*)
-        try congruence;
-         repeat case_match';
-        basic_goal_prep;
-        try congruence;
-        repeat lazymatch goal with
-        | [H : default = Some _ |- _ ] => safe_invert H
-        | [H : Some _ = Some _ |- _ ] => safe_invert H
-          end;
-         basic_goal_prep;
-           repeat lazymatch goal with
-           | [H : Some (term_eq_result _ _ _) = _,
-                 hist : tree_all node_result_sound _ |- _] =>
-               symmetry in H;
-               eapply hist in H
-           | [H : Some (sort_eq_result _ _) = _,
-                 hist : tree_all node_result_sound _ |- _] =>
-               symmetry in H;
-               eapply hist in H
-           end; simpl in *; eauto with term lang_core.
-       - constructor; constructor.
-         apply named_list_lookup_err_in; auto.
-       - safe_invert HeqH2; subst.
-         eapply term_con_congruence; eauto.
-         + apply named_list_lookup_err_in; eauto.
-         + eapply check_args_proof_sound; eauto.
-       - eapply eq_term_subst.
-         3: eapply eq_term_by;
-         apply named_list_lookup_err_in; eauto.
-         + apply named_list_lookup_err_in in HeqH.
-           use_rule_in_wf.
-           inversion H; subst.
-           basic_utils_crush.
-         + eapply eq_args_implies_eq_subst.
-           eapply check_args_proof_sound; eauto.
-       - safe_invert HeqH2; subst.
-         eapply sort_con_congruence; eauto.
-         + apply named_list_lookup_err_in; eauto.
-         + eapply check_args_proof_sound; eauto.
-       - eapply eq_sort_subst.
-         3: eapply eq_sort_by;
-         apply named_list_lookup_err_in; eauto.
-         + apply named_list_lookup_err_in in HeqH.
-           use_rule_in_wf.
-           inversion H; subst.
-           basic_utils_crush.
-         + eapply eq_args_implies_eq_subst.
-           eapply check_args_proof_sound; eauto.
-     Qed.
-  End Inner.
-
-  (*TODO: use named_list for pf instead of list?*)
-  Fixpoint check_proof' (p : pf) : option (tree node_result * positive) :=
-    match p with
-    | [] => Some (empty _, 1%positive)
-    | n::p' =>
-        @! let (p_res, next) <- check_proof' p' in
-           let n_res <- check_node p_res n in
-           ret (set next n_res p_res, next + 1)%positive
-    end.
-
-  Definition check_proof (p : pf) : option (term * term * sort) :=
-    @! let (m, next) <- check_proof' p in
-      let (term_eq_result e1 e2 t) <?- get (next - 1)%positive m in
-      ret (e1,e2,t).
-
-      Require Import Lia.
-      Open Scope positive.
-  
-  Lemma check_proof'_fresh' p res next
-    : check_proof' p = Some (res, next) ->
-      forall n', n' >= next ->
-      get n' res = None.
-  Proof.
-    revert res next; induction p;
-      unfold tree_all;
-      basic_goal_prep;
-      repeat lazymatch goal with
-        | [H : default = Some _ |- _ ] => safe_invert H
-        | [H : Some _ = Some _ |- _ ] => safe_invert H
-        end;
-      basic_goal_prep;
-      eauto;
-      repeat case_match';
-      basic_goal_prep;
-      try congruence.
-    safe_invert H.
-    rewrite gso by lia.
-    eapply IHp; eauto; lia.
-  Qed.
-  
-  Lemma check_proof'_fresh p res next
-    : check_proof' p = Some (res, next) ->
-      get next res = None.
-  Proof.
-    intros; eapply check_proof'_fresh'; eauto; lia.
-  Qed.
-    
-  Lemma check_proof'_sound p res next
-    : check_proof' p = Some (res, next) ->
-      tree_all node_result_sound res.
-  Proof.
-    revert res next; induction p;
-      unfold tree_all;
-      basic_goal_prep;
-        repeat lazymatch goal with
-        | [H : default = Some _ |- _ ] => safe_invert H
-        | [H : Some _ = Some _ |- _ ] => safe_invert H
-          end;
-      basic_goal_prep;
-      eauto using check_node_sound;
-    repeat case_match';
-      basic_goal_prep;
-      try congruence.
-    safe_invert H; simpl.
-    safe_invert HeqH0.
-    destruct (Pos.eq_dec n p0).
-    {
-      subst.
-      rewrite gss in H0.
-      safe_invert H0.
-      eapply check_node_sound; eauto.      
-    }
-    rewrite gso in H0; eauto.
-    eapply IHp; eauto.
-  Qed.
-
-  Theorem check_proof_sound p e1 e2 t
-    : check_proof p = Some (e1,e2,t) ->
-      eq_term l c t e1 e2.
-  Proof.
-    unfold check_proof.
-    remember (check_proof' p) as check.
-    destruct check; simpl; try congruence.
-    destruct p0; simpl; try congruence.
-    repeat case_match;
-      basic_goal_prep;
-        repeat lazymatch goal with
-        | [H : default = Some _ |- _ ] => safe_invert H
-        | [H : Some _ = Some _ |- _ ] => safe_invert H
-          end;
-      try congruence.
-    symmetry in Heqcheck.
-    apply check_proof'_sound in Heqcheck.
-    simpl in *.
-    symmetry in HeqH.
-    specialize (Heqcheck _ _ HeqH).
-    eauto.
-  Qed.
-   *)
-
+      End WithCtx.
   End WithLang.
 
 End WithVar.
